\documentclass[newpage]{homework}
\newcommand{\hwname}{Zooey Nguyen}
\newcommand{\hwemail}{zooeyn@ucla.edu}
\newcommand{\hwclass}{Math 151A}
\newcommand{\hwtype}{Homework}
\newcommand{\hwnum}{6}
\begin{document}
\maketitle

\question
Backwards difference approximations for derivative of $\sin x$ at $x = \pi/3$. Note $(\sin x)'|_{x=\pi/3} = \cos(\pi/3) = 0.5$. The error decreases by about a factor of 10 each time.
\begin{align*}
	f'(\pi/3)	&\approx	\frac{\sin(\pi/3)-\sin(\pi/3-0.1)}{0.1}	= 0.54243	&
	e_{abs} &= 0.04243 \\
	f'(\pi/3)	&\approx	\frac{\sin(\pi/3)-\sin(\pi/3-0.01)}{0.01}	= 0.50432	&
	e_{abs} &= 0.00432 \\
	f'(\pi/3)	&\approx	\frac{\sin(\pi/3)-\sin(\pi/3-0.001)}{0.001}	= 0.50043	&
	e_{abs} &= 0.00043 \\
\end{align*}

\question
Formula with $h/2$.
\begin{align*}
	f'(x_0)	&=	\frac{f(x_0+\frac{h}{2})-f(x_0-\frac{h}{2})}{h} - \left(\frac{h^2}{24} f'''(x_0) + \frac{h^4}{1920} f^{(5)}(\xi)  \right)
\end{align*}
New approximation.
\begin{align*}
	4f'(x_0)	&=	4\frac{f(x_0+\frac{h}{2})-f(x_0-\frac{h}{2})}{h} - \left(\frac{h^2}{6} f'''(x_0) + \frac{h^4}{480} f^{(5)}(\xi)  \right)	\\
	3f'(x_0)	&=	4\frac{f(x_0+\frac{h}{2})-f(x_0-\frac{h}{2})}{h} - \left(\frac{h^2}{6} f'''(x_0) + \frac{h^4}{480} f^{(5)}(\xi)  \right) - \frac{f(x_0+h)-f(x_0-h)}{4h} + \left(\frac{h^2}{6} f'''(x_0) + \frac{h^4}{120} f^{(5)}(\xi)  \right)	\\
	&=	4\frac{f(x_0+\frac{h}{2})-f(x_0-\frac{h}{2})}{h} - \frac{f(x_0+h)-f(x_0-h)}{4h} - \frac{3h^4}{480} f^{(5)}(\xi)	\\
	&=	\frac{16f(x_0+\frac{h}{2})-16f(x_0-\frac{h}{2})-f(x_0+h)-f(x_0-h)}{4h} - \frac{3h^4}{480} f^{(5)}(\xi)	\\
	f'(x_0)	&=	\frac{16f(x_0+\frac{h}{2})-16f(x_0-\frac{h}{2})-f(x_0+h)-f(x_0-h)}{12h} - \boxed{\frac{h^4}{480} f^{(5)}(\xi)}
\end{align*}

\question
Taylor expansion at $x_1$.
\begin{align*}
	f(x)	&=	f(x_1) + f'(x_1)(x-x_1) + \frac{f''(x_1)}{2!}(x-x_1)^2 + \frac{f^{(3)}(x_1)}{3!}(x-x_1)^3 + \frac{f^{(4)}(\xi)}{4!}(x-x_1)^4
\end{align*}
Integral of Taylor expansion at $x_1$ on $x_0, x_2$.
\begin{align*}
	\int_{x_0}^{x_2} f(x) \dd{x}	&=	\int_{x_0}^{x_2} f(x_1) + f'(x_1)(x-x_1) + \frac{f''(x_1)}{2!}(x-x_1)^2 + \frac{f^{(3)}(x_1)}{3!}(x-x_1)^3 + \frac{f^{(4)}(\xi)}{4!}(x-x_1)^4 \dd{x}	\\
	&=	f(x_1)x\Big|_{x_0}^{x_2} + f'(x_1)\frac{(x-x_1)^2}{2}\Big|_{x_0}^{x_2} + \frac{f''(x_1)}{2!}\frac{(x-x_1)^3}{3}\Big|_{x_0}^{x_2} + \frac{f^{(3)}(x_1)}{3!}\frac{(x-x_1)^4}{4}\Big|_{x_0}^{x_2} + \frac{1}{24} \int_{x_0}^{x_2} f^{(4)}(\xi) (x-x_1)^4 \dd{x}	\\
	&=	f(x_1)(x_2-x_0) + \frac{f''(x_1)}{2!}\frac{(x_2-x_1)^3 - (x_0-x_1)^3}{3}	+ \frac{1}{24} \int_{x_0}^{x_2} f^{(4)}(\xi) (x-x_1)^4 \dd{x} \\
	&=	2hf(x_1) + \frac{f''(x_1)}{2!}\frac{h^3 + h^3}{3}	+ \frac{1}{24} \int_{x_0}^{x_2} f^{(4)}(\xi) (x-x_1)^4 \dd{x} \\
	&=	2hf(x_1) + \frac{h^3}{3}f''(x_1)	+ \frac{1}{24} \int_{x_0}^{x_2} f^{(4)}(\xi) (x-x_1)^4 \dd{x} \\
\end{align*}

\question


\end{document}
